Simple_Clause_Learning/Non_Redundancy.thy
@@ -1849,7 +1849,7 @@ proof -
           ground_conf: "is_ground_cls (add_mset L C \<cdot> \<gamma>\<^sub>C)" and
           ground_reso: "is_ground_cls (add_mset K D \<cdot> \<gamma>\<^sub>D)" and
           dom_\<gamma>\<^sub>C: "subst_domain \<gamma>\<^sub>C \<subseteq> vars_cls (add_mset L C)" and
-          dom_\<gamma>\<^sub>D: "subst_domain \<gamma>\<^sub>D \<subseteq> vars_cls (add_mset K D)" and
+          (* dom_\<gamma>\<^sub>D: "subst_domain \<gamma>\<^sub>D \<subseteq> vars_cls (add_mset K D)" and *)
           "sound_trail N \<Gamma>"
           unfolding sound_state_def \<open>\<Gamma> = trail_propagate \<Gamma>' K D \<gamma>\<^sub>D\<close>
           by (simp_all add: minimal_ground_closures_def propagate_lit_def)
@@ -1889,7 +1889,7 @@ proof -
         qed
         hence "trail_false_cls (state_trail S1) ((C \<cdot> \<rho>\<^sub>C + D \<cdot> \<rho>\<^sub>D) \<cdot> \<mu> \<cdot>
           (rename_subst_domain \<rho>\<^sub>C \<gamma>\<^sub>C \<odot> rename_subst_domain \<rho>\<^sub>D \<gamma>\<^sub>D))"
-          using imgu_idempotent_on_renamed_comp_renamed[OF _ dom_\<gamma>\<^sub>C dom_\<gamma>\<^sub>D ground_conf ground_reso]
+          using imgu_idempotent_on_renamed_comp_renamed[OF _ dom_\<gamma>\<^sub>C ground_conf ground_reso]
           using resolveI(3-)
           by (metis is_renaming_iff subst_cls_comp_subst)
         hence "trail_false_cls (state_trail S1) ((C \<cdot> \<rho>\<^sub>C + D \<cdot> \<rho>\<^sub>D) \<cdot> \<mu> \<cdot> \<gamma>)"
